##### 5.15

C

##### 5.16

(1)
$$
H(D) = -\sum_{i=1}^{n}p(x_i)logp(x_i)\\
=-\frac{4}{9}log\frac{4}{9}-\frac{5}{9}log\frac{5}{9}\\
=\frac{4}{9}log\frac{9}{4}+\frac{5}{9}log\frac{9}{5}\\
$$
(2)

由
$$
H(D)=\frac{4}{9}log\frac{9}{4}+\frac{5}{9}log\frac{9}{5}\\
H(D|a_1)=\frac{4}{9}(-\frac{3}{4}log\frac{3}{4}-\frac{1}{4}log\frac{1}{4})+\frac{5}{9}(-\frac{1}{5}log\frac{1}{5}-\frac{4}{5}log\frac{4}{5})\\
H(D|a_2)=\frac{5}{9}(-\frac{2}{5}log\frac{2}{5}-\frac{3}{5}log\frac{3}{5})+\frac{4}{9}(-\frac{2}{4}log\frac{2}{4}-\frac{2}{4}log\frac{2}{4})\\
H(D|a_3)=\frac{4}{9}(-\frac{3}{4}log\frac{3}{4}-\frac{1}{4}log\frac{1}{4})+\frac{5}{9}(-\frac{1}{5}log\frac{1}{5}-\frac{4}{5}log\frac{4}{5})\\
$$
所以$a_1,a_2,a_3$的信息增益分别是
$$
H(D)-H(D|a_1)\\
H(D)-H(D|a_2)\\
H(D)-H(D|a_3)
$$

##### 5.17

B,C,D





